theories/L4_deBruijn/L4_to_L4a_correct.v
@@ -1,0 +1,275 @@
+Require Import L4.expression.
+Require Import L4.L4a_to_L5.
+Require Import L4.L4_to_L4a.
+
+Require Import SquiggleEq.export.
+Require Import SquiggleEq.UsefulTypes.
+Require Import SquiggleEq.varImplZ.
+
+(* circularity watch: this correctness property cannot go to L4.instances. Should we have
+L4.correctnessInstances for such instances? *)
+Require Import L4.instances.
+Require Import Common.certiClasses.
+
+Require Import BinNat.
+Require Import BinPos.
+Require Import Omega.
+Require Import Psatz.
+Require Import Arith.
+Require Import PArith.
+Require Import NArith.
+
+
+(*
+Lemma mkVarPreservesLt (a b : N) : (a < b)%N -> (mkVar a < mkVar b)%positive.
+Proof.
+  intro H.
+  unfold mkVar.
+  unfold Pos.lt.
+  rewrite Pos.compare_xO_xO.
+  fold (Pos.lt (N.succ_pos a) (N.succ_pos b)).
+  (* Obvious! Perhaps we should use MathClasses to 
+        avoid hunting aroung Coq's standard library*)
+Admitted.
+*)
+
+Require Import SquiggleEq.tactics.
+Print my_exp_wf_ind.
+Require Import Basics.
+SearchAbout Basics.compose. 
+Require Import Coq.Unicode.Utf8.
+Require Import List.
+Require Import SquiggleEq.list.
+
+
+Open Scope program_scope.
+Print exp_wf.
+Lemma L4_to_L4a_fvars: 
+  (forall n (s : exp),
+    L4.expression.exp_wf n s 
+    -> forall v, List.In v (free_vars (L4_to_L4a n s)) -> 
+        (Npos (Pos.div2 v) < N.succ n)%N /\ varClass v = true (* user variable *))
+ ∧
+  (forall n (s : exps),
+    L4.expression.exps_wf n s 
+    -> forall v, List.In v (flat_map free_vars (translatel mkVar n s)) -> 
+        (Npos (Pos.div2 v) < N.succ n)%N /\ varClass v = true (* user variable *))
+ ∧
+  (forall n (s : efnlst),
+    L4.expression.efnlst_wf n s 
+    -> forall v, List.In v (flat_map free_vars (translatef mkVar n s)) -> 
+        (Npos (Pos.div2 v) < N.succ n)%N /\ varClass v = true (* user variable *))
+ ∧
+  (forall n (s : branches_e),
+    L4.expression.branches_wf n s 
+    -> forall v, List.In v (flat_map (free_vars_bterm ∘ snd)  (translateb mkVar n s)) -> 
+        (Npos (Pos.div2 v) < N.succ n)%N /\ varClass v = true (* user variable *))
+.
+Proof.
+  apply my_exp_wf_ind;
+  intros ? ?.
+- intros Hwf ? Hin. simpl in Hin. rewrite or_false_r in Hin.
+  subst. split; [ | refl].
+  simpl.
+  rewrite N.succ_pos_spec.
+  rewrite N.sub_1_r.
+  rewrite N.lt_succ_pred with (z:=0%N); lia.
+
+- intros Hwf Hind ? Hin.
+  simpl in Hin. fold (L4_to_L4a.translate mkVar (N.succ i)) in Hin.
+  rewrite list.in_app_iff in Hin.
+  rewrite or_false_r in Hin.
+  apply list.in_remove in Hin.
+  repnd. rewrite  N.add_1_l in Hind.
+  apply Hind in Hin.
+  clear Hind. rename Hin into Hind.
+  repnd.
+  split; [ | assumption].
+  apply N.lt_succ_r in Hind0.
+  apply N.lt_eq_cases in Hind0.
+  dorn Hind0; [assumption | subst; provefalse ].
+  apply Hin0.
+  clear Hin0.
+  destruct v; inversion Hind. clear Hind.
+  simpl in Hind0.
+  unfold mkVar. 
+  f_equal.
+  rewrite <- N.succ_pos_spec in Hind0.
+  injection Hind0. trivial.
+
+- intros ? ? H1ind H1wf H2ind ? Hin. simpl in Hin.
+  fold (L4_to_L4a.translate mkVar i) in Hin.
+  repeat (rewrite list.in_app_iff in Hin).
+  rewrite or_false_r in Hin.
+  dorn Hin; eauto.
+
+- intros ? Hwf Hind ? Hin.
+  simpl in Hin.
+  fold (L4_to_L4a.translatel mkVar i) in Hin.
+  rewrite flat_map_bterm_nil in Hin.
+  eauto.
+
+- intros ? ? Hwf Hind ? Hindb ? Hin.
+  simpl in Hin.
+  fold (L4_to_L4a.translateb mkVar i) in Hin.
+  fold (L4_to_L4a.translate mkVar i) in Hin.
+  apply list.in_app_iff in Hin.
+  rewrite list.flat_map_map in Hin.
+  dorn Hin; eauto.
+
+- intros ? Hwf Hind H2wf H2ind ? Hin.
+  simpl in Hin.
+  fold (L4_to_L4a.translate mkVar (N.succ i)) in Hin.
+  fold (L4_to_L4a.translate mkVar i) in Hin.
+  repeat rewrite list.in_app_iff in Hin.
+  simpl in Hin.
+  rewrite or_false_r in Hin.
+  dorn Hin;[eauto; fail | ].
+  clear Hind Hwf. rename H2ind into Hind.
+  apply list.in_remove in Hin.
+  repnd. rewrite  N.add_1_l in Hind.
+  apply Hind in Hin.
+  clear Hind. rename Hin into Hind.
+  repnd.
+
+  (* the part below is a suffix of the lambda case *)
+  split; [ | assumption].
+  apply N.lt_succ_r in Hind0.
+  apply N.lt_eq_cases in Hind0.
+  dorn Hind0; [assumption | subst; provefalse ].
+  apply Hin0.
+  clear Hin0.
+  destruct v; inversion Hind. clear Hind.
+  simpl in Hind0.
+  unfold mkVar.
+  f_equal.
+  rewrite <- N.succ_pos_spec in Hind0.
+  injection Hind0. trivial.
+
+- intros ? Hwf Hind ? Hin.
+  simpl in Hin.
+  fold (L4_to_L4a.translatef  mkVar (N.succ i)) in Hin.
+
+Print exp_wf.
+Print sbst_fix. 
+
+Print exp_wf.
+(*  rewrite flat_map_bterm_nil in Hin.
+  rwsimpl Hin.
+   
+  eauto.
+compute in Hin. *)
+Abort.
+
+
+Lemma L4_to_L4a_preserves_wf : 
+  certiClasses.wfPreserving (cTerm certiL4) (cTerm certiL4a).
+Proof.
+  intros ? ?. simpl. unfold wf. unfold WellFormed_instance_1.
+  compute in s.
+  compute in H.
+Abort.
+
+Print Nat.even.
+Fixpoint isEven (n:nat) : bool := 
+match n with
+| 0 => true
+| S n' => isOdd n' (* && isEven n' *)
+end
+with isOdd (n:nat) : bool :=
+match n with
+| 0 => false
+| S n' => isEven n' (* && isOdd n' *)
+end.
+
+Quote Recursively Definition isEven3 := (isEven 3).
+
+(* Move to an earlier file because it is more generally useful *)
+Ltac cexact x := let t := eval compute in x in exact t.
+Require Import L2.instances.
+
+Definition isEven3L4 := ltac:(cexact (translateTo (cTerm certiL4) isEven3)).
+
+Open Scope string_scope.
+Print isEven3.
+
+Local Opaque Match_e.
+Local Opaque Fix_e.
+Local Opaque Proj_e.
+Local Opaque Con_e.
+Local Opaque Lam_e.
+Local Opaque Let_e.
+Local Opaque App_e.
+
+Local Transparent ssubst_aux.
+Local Transparent ssubst_bterm_aux.
+Definition isEven3L4a := ltac:(cexact (translateTo (cTerm certiL4a) isEven3)).
+
+Print isEven3L4.
+Print isEven3L4a.
+
+Eval vm_compute in isEven3L4a.
+
+Eval compute in (DecidableClass.decide (2=3))%positive.
+
+
+
+Require Import L4.expression.
+Require Import Common.Common.
+
+Hint Constructors expression.eval.
+Hint Constructors expression.evals.
+Lemma isEven3Eval : exists v, isEven3L4 ⇓ v.
+Proof.
+  compute.
+  evar (v: (cTerm certiL4)).
+  exists (Ret v).
+  econstructor; eauto.
+  compute.
+  try (econstructor; eauto;compute;[]).
+  eapply expression.eval_FixApp_e; try (compute; eauto; fail);
+    [apply eval_Con_e; repeat (econstructor; eauto) | ].
+(* Constructors are numbered as listed in Coq definition : e.g. 0 for O and 1 for S --
+see how 3 gets represented.
+
+In Template Coq, [(tConstruct (mkInd "Coq.Init.Datatypes.nat" 0) 1)] 
+the "1" at the end represents "S". The "0" perhaps signifies that this constructor
+is one of the first inductive block in the (trivially)mutually inductive block.
+
+
+Var_e 2  revers to isOdd. in the sibling of the branch where 
+Var_e 2 is mentioned, true is returned in the other case. 
+Var_e 3  revers to isEven.
+
+In a nominal (w.r.t. variable bindings) setting,
+ this ordering is reverse of how these definitions appear in the mutually inductive block.
+However, note that these are DB indices. So, the highest number is the outermost (head) 
+of the list of fix bodies, which is isEven. So it makes sense in the DB setting.
+
+Also, note how sbst_fix accounts for this by folding over the list of indices in a 
+decreasing order. Also, note that this choice of reverse ordering goes back to Template Coq--
+see isEven3
+
+*)
+  unfold sbst_fix.
+  simpl list_to_zero.
+  remember (0%nat :: nil) as l0.
+  simpl.
+  compute.
+  subst l0. compute.
+  econstructor; eauto;
+    [apply eval_Con_e; repeat (econstructor; eauto) | ].
+  compute.
+  econstructor; eauto;
+    [apply eval_Con_e; repeat (econstructor; eauto) | | ].
+  compute.
+  econstructor; eauto.
+  compute.
+  eapply expression.eval_FixApp_e; try (compute; eauto; fail);
+    [apply eval_Con_e; repeat (econstructor; eauto) | ].
+  compute.
+  compute.
+Abort.
+
+
+
